apc/APCA.v
@@ -6,7 +6,7 @@ Set Implicit Arguments.
 
 Module APCA. Section APCA.
   Import APC.
-  Context `{!invG α Σ Γ, !subG Γ Σ, !sinvG Σ Γ α β τ}.
+  Context `{_sinvG: !sinvG Γ Σ α β τ _I _S}.
 
   Definition scopes := ["APC"].
 
